theories/Array/Array.v
@@ -1,30 +1,92 @@
-Require Export ArrayOp.
-Require Export Cyclic31.
+Require Export Int31.
+
+Register array : Type -> Type as array_type.
+
+Register make : forall {A:Type}, int -> A -> array A as array_make.
+
+Register get : forall {A:Type}, array A -> int -> A as array_get.
+Register default : forall {A:Type}, array A -> A as array_default.
+
+Register set : forall {A:Type}, array A -> int -> A -> array A as array_set.
+
+Register length : forall {A:Type}, array A -> int as array_length.
+
+Register copy : forall {A:Type}, array A -> array A as array_copy.
+
+Register reroot : forall {A:Type}, array A -> array A as array_reroot.
+
+Delimit Scope array_scope with array.
+Notation "t '.[' i ']'" := (get t i) (at level 50) : array_scope.
+Notation "t '.[' i '<-' a ']'" := (set t i a) (at level 50) : array_scope.
 
 Local Open Scope int31_scope.
-Local Open Scope bool_scope.
+Local Open Scope array_scope.
 
 Set Vm Optimize.
 
-Definition to_list (A:Type) (t:array A) :=
-  let len := length _ t in
+Definition max_array_length := 4194302.
+
+(** Axioms *)
+Axiom get_outofbound : forall A (t:array A) i, (i < length t) = false -> t.[i] = default t.
+
+Axiom get_set_same : forall A t i (a:A), (i < length t) = true -> t.[i<-a].[i] = a.
+Axiom get_set_other : forall A t i j (a:A), i <> j -> t.[i<-a].[j] = t.[j].
+
+Axiom get_make : forall A (a:A) size i, (make size a).[i] = a.
+Axiom default_make : forall A (a:A) size, (default (make size a)) = a.
+
+(*** TODO: remove this axiom using get_outofbound, get_set_other *)
+Axiom default_set : forall A t i (a:A),
+  default (t.[i<-a]) = default t.
+
+Axiom length_make : forall A size (a:A), 
+  length (make size a) = if size <= max_array_length then size else max_array_length.
+Axiom length_set : forall A t i (a:A),
+  length (t.[i<-a]) = length t.
+
+Axiom copy_get : forall A (t:array A) i, (copy t).[i] = t.[i].
+Axiom copy_length : forall A (t:array A), length (copy t) = length t.
+(*** TODO: remove this axiom using get_outofbound, copy_get *)
+Axiom copy_default : forall A (t:array A), default (copy t) = default t.
+
+Axiom reroot_get : forall A (t:array A) i, (reroot t).[i] = t.[i].
+Axiom reroot_length : forall A (t:array A), length (copy t) = length t.
+(*** TODO: remove this axiom using get_outofbound, reroot_get *)
+Axiom reroot_default : forall A (t:array A), default (copy t) = default t.
+
+
+Definition to_list {A:Type} (t:array A) :=
+  let len := length t in
   if len == 0 then nil
-  else foldi_down _ (fun i l => get _ t i :: l)%list (len - 1) 0 nil.
+  else foldi_down (fun i l => t.[i] :: l)%list (len - 1) 0 nil.
 
-Definition forallb (A:Type) (f:A->bool) (t:array A) :=
-  let len := length _ t in
-  if len == 0 then true
-  else
-    foldi_cont31 _ _ (fun i (cont:unit -> bool) (_:unit) =>
-      if f (get _ t i) then cont tt else false) 0 (length _ t - 1) 
-    (fun _ => true) tt.
+Definition forallb {A:Type} (f:A->bool) (t:array A) :=
+  forallb (fun i => f (t.[i])) 0 (length t - 1).
 
-Definition existsb (A:Type) (f:A->bool) (t:array A) :=
-  let len := length _ t in
-  if len == 0 then false
-  else
-    foldi_cont31 _ _ (fun i (cont:unit -> bool) (_:unit) =>
-         if f (get _ t i) then true else cont tt) 0 (length _ t - 1)
-    (fun _ => false) tt.
+Definition existsb {A:Type} (f:A->bool) (t:array A) :=
+  existsb (fun i => f (t.[i])) 0 (length t - 1).
+
+Definition mapi {A B:Type} (f:int->A->B) (t:array A) :=
+  let size := length t in
+  let def := f size (default t) in
+  let tb := make size def in
+  foldi (fun i tb => tb.[i<- f i (t.[i])]) 0 (size - 1) tb.
+
+Definition map {A B:Type} (f:A->B) :=
+  Eval lazy beta delta [mapi] in (mapi (fun i => f)).
+
+Definition foldi_left {A B:Type} (f:int -> A -> B -> A) a (t:array B) :=
+  foldi (fun i a => f i a (t.[i])) 0 (length t - 1) a.
+
+Definition fold_left {A B:Type} (f: A -> B -> A) a (t:array B) :=
+  foldi (fun i a => f a (t.[i])) 0 (length t - 1) a.
+
+Definition foldi_right {A B:Type} (f:int -> A -> B -> B) (t:array A) b :=
+  foldi_down (fun i b => f i (t.[i]) b) (length t - 1) 0 b.
+
+Definition fold_right {A B:Type} (f: A -> B -> B) (t:array A) b :=
+  foldi_down (fun i b => f (t.[i]) b) (length t - 1) 0 b.
+
+
 
 
