theories/Numbers/Cyclic/Int31/Int31Op.v
@@ -8,144 +8,164 @@
 (************************************************************************)
 (*            Benjamin Gregoire, Laurent Thery, INRIA, 2007             *)
 (************************************************************************)
-
-Require Import BigNumPrelude.
 Require Export Int31Native.
+Require Import BigNumPrelude.
+Require Import Bvector.
 
 Set Vm Optimize.
 
 
 Local Open Scope int31_scope.
-Local Open Scope bool_scope.
 
-(** The number of digits as a int31 *)
+(** The number of digits as a int *)
 Definition digits := 31.
 
 (** The bigger int *)
-Definition max_int31 := Eval compute in 0 - 1.
-Register max_int31 as Inline.
+Definition max_int := Eval compute in 0 - 1.
+Register max_int as Inline.
 
 (** Access to the nth digits *)
 Definition get_digit x p := (0 < (x land (1 << p))).
 
 Definition set_digit x p (b:bool) :=
-  if (0 <= p) && (p < 31) then 
+  if (0 <= p) && (p < digits) then 
     if b then x lor (1 << p)
-    else x land (max_int31 lxor (1 << p))
+    else x land (max_int lxor (1 << p))
   else x.
 
 (** Equality to 0 *)
-Definition is_zero (i:int31) := i == 0.
+Definition is_zero (i:int) := i == 0.
 Register is_zero as Inline.
 
 (** Parity *)
-Definition is_even (i:int31) := is_zero (i land 1).
+Definition is_even (i:int) := is_zero (i land 1).
 Register is_even as Inline.
 
 (** Extra modulo operations *)
-Definition opp31 (i:int31) := 0 - i.
-Register opp31 as Inline.
-Notation "- x" := (opp31 x) : int31_scope.
+Definition opp (i:int) := 0 - i.
+Register opp as Inline.
+Notation "- x" := (opp x) : int31_scope.
 
-Definition opp31carry i := max_int31 - i.
-Register is_zero as Inline.
+Definition oppcarry i := max_int - i.
+Register oppcarry as Inline.
 
-Definition succ31 i := i + 1.
-Register opp31carry as Inline.
+Definition succ i := i + 1.
+Register succ as Inline.
 
-Definition pred31 i := i - 1.
-Register pred31 as Inline.
+Definition pred i := i - 1.
+Register pred as Inline.
 
-Definition add31carry i j := i + j + 1.
-Register add31carry as Inline.
+Definition addcarry i j := i + j + 1.
+Register addcarry as Inline.
 
-Definition sub31carry i j := i - j - 1.
-Register sub31carry as Inline.
+Definition subcarry i j := i - j - 1.
+Register subcarry as Inline.
 
 (** Exact arithmetic operations *)
 
-Definition add31c_def x y :=
+Definition addc_def x y :=
   let r := x + y in
   if r < x then C1 r else C0 r.
 (* the same but direct implementation for effeciancy *)
-Register add31c      : int31 -> int31 -> carry int31 as int31_addc.
-Notation "n '+c' m" := (add31c n m) (at level 50, no associativity) : int31_scope.
+Register addc      : int -> int -> carry int as int31_addc.
+Notation "n '+c' m" := (addc n m) (at level 50, no associativity) : int31_scope.
 
-Definition add31carryc_def x y :=
-  let r := add31carry x y in
+Definition addcarryc_def x y :=
+  let r := addcarry x y in
   if r <= x then C1 r else C0 r.
 (* the same but direct implementation for effeciancy *)
-Register add31carryc : int31 -> int31 -> carry int31 as int31_addcarryc.
+Register addcarryc : int -> int -> carry int as int31_addcarryc.
 
-Definition sub31c_def x y := 
+Definition subc_def x y := 
   if y <= x then C0 (x - y) else C1 (x - y).
 (* the same but direct implementation for effeciancy *)
-Register sub31c      : int31 -> int31 -> carry int31 as int31_subc.
-Notation "n '-c' m" := (sub31c n m) (at level 50, no associativity) : int31_scope.
+Register subc      : int -> int -> carry int as int31_subc.
+Notation "n '-c' m" := (subc n m) (at level 50, no associativity) : int31_scope.
 
-Definition sub31carryc_def x y :=
+Definition subcarryc_def x y :=
   if y < x then C0 (x - y - 1) else C1 (x - y - 1).
 (* the same but direct implementation for effeciancy *)
-Register sub31carryc : int31 -> int31 -> carry int31 as int31_subcarryc.
+Register subcarryc : int -> int -> carry int as int31_subcarryc.
 
-Definition diveucl31_def x y := (x/y, x\%y).
+Definition diveucl_def x y := (x/y, x\%y).
 (* the same but direct implementation for effeciancy *) 
-Register diveucl31   : int31 -> int31 -> int31 * int31 as int31_diveucl.
+Register diveucl   : int -> int -> int * int as int31_diveucl.
 
-Register diveucl31_21    : int31 -> int31 -> int31 -> int31 * int31 as int31_div21.
+Register diveucl_21    : int -> int -> int -> int * int as int31_div21.
 
-Definition addmuldiv31_def p x y :=
+Definition addmuldiv_def p x y :=
   (x << p) lor (y >> (digits - p)).
-Register addmuldiv31   : int31 -> int31 -> int31 -> int31 as int31_addmuldiv.
+Register addmuldiv   : int -> int -> int -> int as int31_addmuldiv.
 
-Definition opp31c (i:int31) := 0 -c i.
-Register opp31c as Inline.
+Definition oppc (i:int) := 0 -c i.
+Register oppc as Inline.
 
-Definition succ31c i := i +c 1.
-Register succ31c as Inline.
+Definition succc i := i +c 1.
+Register succc as Inline.
 
-Definition pred31c i := i -c 1.
-Register pred31c as Inline.
+Definition predc i := i -c 1.
+Register predc as Inline.
 
 (** Comparison *)
-Definition compare31_def x y :=
+Definition compare_def x y :=
   if x < y then Lt 
   else if (x == y) then Eq else Gt.
 
-Register compare31 : int31 -> int31 -> comparison as int31_compare.
-Notation "n ?= m" := (compare31 n m) (at level 70, no associativity) : int31_scope.
+Register compare : int -> int -> comparison as int31_compare.
+Notation "n ?= m" := (compare n m) (at level 70, no associativity) : int31_scope.
 
 (** Exotic operations *)
 
-Register head0 : int31 -> int31 as int31_head0.
-Register tail0 : int31 -> int31 as int31_tail0.
+(** I should add the definition (like for compare) *)
+Register head0 : int -> int as int31_head0.
+Register tail0 : int -> int as int31_tail0.
 
 (** Iterators *)
 
-Definition foldi A (f:int31 -> A -> A) from to :=
-  foldi_cont31 A A (fun i cont a => cont (f i a)) from to (fun a => a).
+Definition foldi {A} (f:int -> A -> A) from to :=
+  foldi_cont (fun i cont a => cont (f i a)) from to (fun a => a).
 Register foldi as Inline.
 
-Definition fold A (f: A -> A) from to :=
-  foldi_cont31 A A (fun i cont a => cont (f a)) from to (fun a => a).
+Definition fold {A} (f: A -> A) from to :=
+  foldi_cont (fun i cont a => cont (f a)) from to (fun a => a).
 Register fold as Inline.
 
-Definition foldi_down A (f:int31 -> A -> A) from downto :=
-  foldi_down_cont31 A A (fun i cont a => cont (f i a)) from downto (fun a => a).
+Definition foldi_down {A} (f:int -> A -> A) from downto :=
+  foldi_down_cont (fun i cont a => cont (f i a)) from downto (fun a => a).
 Register foldi_down as Inline.
 
-Definition fold_down A (f:A -> A) from downto :=
-  foldi_down_cont31 A A (fun i cont a => cont (f a)) from downto (fun a => a).
+Definition fold_down {A} (f:A -> A) from downto :=
+  foldi_down_cont (fun i cont a => cont (f a)) from downto (fun a => a).
 Register fold_down as Inline.
 
-Definition forallb (f:int31 -> bool) from to :=
-  foldi_cont31 _ bool (fun i cont _ => if f i then cont tt else false) from to (fun _ => true) tt.
+Definition forallb (f:int -> bool) from to :=
+  foldi_cont (fun i cont _ => if f i then cont tt else false) from to (fun _ => true) tt.
 
-Definition existsb (f:int31 -> bool) from to :=
-  foldi_cont31 _ bool (fun i cont _ => if f i then true else cont tt) from to (fun _ => false) tt.
+Definition existsb (f:int -> bool) from to :=
+  foldi_cont (fun i cont _ => if f i then true else cont tt) from to (fun _ => false) tt.
+
+(** Translation to Bvector *)
+
+Fixpoint to_vect_rec (n:nat) (i:int) : Bvector n :=
+  match n as n0 return Bvector n0 with
+  | O => Bnil
+  | S n' => Bcons (negb (is_even i)) n' (to_vect_rec n' (i>>1))
+  end.
+
+Definition to_vect := to_vect_rec size.
+
+Fixpoint of_vect_rec (n:nat) : Bvector n -> int :=
+ match n as n0 return Bvector n0 -> int with
+ | O => fun _ => 0
+ | S n' => fun v => 
+   (if Blow n' v then fun x => x lor 1 else fun x => x) ((of_vect_rec n' (Bhigh n' v)) << 1)
+ end.
+
+Definition of_vect := of_vect_rec size.
 
 (** Translation to Z *)
-Fixpoint to_Z_rec (n:nat) (i:int31) :=
+
+Fixpoint to_Z_rec (n:nat) (i:int) :=
   match n with 
   | O => 0%Z 
   | S n => 
@@ -172,191 +192,68 @@ Definition of_Z z :=
   end.
 
 (** Gcd **)
-Fixpoint gcd31_rec (guard:nat) (i j:int31) {struct guard} :=
+Fixpoint gcd_rec (guard:nat) (i j:int) {struct guard} :=
    match guard with
    | O => 1
-   | S p => if j == 1 then i else gcd31_rec p j (i \% j)
+   | S p => if j == 0 then i else gcd_rec p j (i \% j)
    end.
 
-Definition gcd31 := gcd31_rec (2*size).
+Definition gcd := gcd_rec (2*size).
 
 (** Square root functions using newton iteration **)
 
-Definition sqrt31_step (rec: int31 -> int31 -> int31) (i j: int31)  :=
+Definition sqrt_step (rec: int -> int -> int) (i j: int)  :=
   let quo := i/j in
   if quo < j then rec i ((j + i/j) >> 1)
   else j.
 
-Definition iter31_sqrt :=
- Eval lazy beta delta [sqrt31_step] in
- fix iter31_sqrt (n: nat) (rec: int31 -> int31 -> int31)
-          (i j: int31) {struct n} : int31 :=
-  sqrt31_step
+Definition iter_sqrt :=
+ Eval lazy beta delta [sqrt_step] in
+ fix iter_sqrt (n: nat) (rec: int -> int -> int)
+          (i j: int) {struct n} : int :=
+  sqrt_step
    (fun i j => match n with
       O =>  rec i j
-   | S n => (iter31_sqrt n (iter31_sqrt n rec)) i j
+   | S n => (iter_sqrt n (iter_sqrt n rec)) i j
    end) i j.
 
-Definition sqrt31 i :=
-  match compare31 1 i with
+Definition sqrt i :=
+  match compare 1 i with
     Gt => 0
   | Eq => 1
-  | Lt => iter31_sqrt 31 (fun i j => j) i (i >> 1)
+  | Lt => iter_sqrt size (fun i j => j) i (i >> 1)
   end.
 
-Definition sqrt312_step (rec: int31 -> int31 -> int31 -> int31)
-   (ih il j: int31)  :=
+Definition sqrt2_step (rec: int -> int -> int -> int)
+   (ih il j: int)  :=
   if ih < j then
-    let (quo,_) := diveucl31_21 ih il j in
+    let (quo,_) := diveucl_21 ih il j in
     if quo < j then
-      let m := 
-        match j +c quo with
-        | C0 m1 => m1 >> 1
-        | C1 m1 => (m1 >> 1) + 30
-        end in 
-      rec ih il m
+      match j +c quo with
+      | C0 m1 => rec ih il (m1 >> 1)
+      | C1 m1 => rec ih il ((m1 >> 1) + 30)
+      end 
     else j
   else j.
 
-Definition iter312_sqrt :=
- Eval lazy beta delta [sqrt312_step] in
- fix iter312_sqrt (n: nat)
-          (rec: int31  -> int31 -> int31 -> int31)
-          (ih il j: int31) {struct n} : int31 :=
-  sqrt312_step
+Definition iter2_sqrt :=
+ Eval lazy beta delta [sqrt2_step] in
+ fix iter2_sqrt (n: nat)
+          (rec: int  -> int -> int -> int)
+          (ih il j: int) {struct n} : int :=
+  sqrt2_step
    (fun ih il j => 
      match n with
      | O =>  rec ih il j
-     | S n => (iter312_sqrt n (iter312_sqrt n rec)) ih il j
+     | S n => (iter2_sqrt n (iter2_sqrt n rec)) ih il j
    end) ih il j.
 
-Definition sqrt312 ih il :=
-  let s := iter312_sqrt 31 (fun ih il j => j) ih il max_int31 in
-  let (ih1, il1) := mul31c s s in
+Definition sqrt2 ih il :=
+  let s := iter2_sqrt size (fun ih il j => j) ih il max_int in
+  let (ih1, il1) := mulc s s in
   match il -c il1 with
   | C0 il2 =>
     if ih1 < ih then (s, C1 il2) else (s, C0 il2)
   | C1 il2 =>
     if ih1 < (ih - 1) then (s, C1 il2) else (s, C0 il2)
   end.
-
-
-(*
-Require Import Int31Bool.
-Print to_Z.
-Check get_digit.
-Print Int31_to_Z.
-
-Fixpoint to_Z2_aux (n:nat) (x:int31) z := 
- match n with
- | O => z
- | S n' =>
-   to_Z2_aux n' x (Zdigit_of_bool (get_digit x (of_Z (Z_of_nat n'))) z)
- end.
-
-Definition to_Z2 x := to_Z2_aux size x Z0.
-
-Require Import Bvector.
-Print Module Bvector.
-Print Bvector.
-Fixpoint to_bvect (n:nat) (x:int31) : Bvector n :=
- match n as n0 return Bvector n0 with
- | O => Bnil
- | S n' => Bcons (get_digit x (of_Z (Z_of_nat n'))) n' (to_bvect n' x)
- end.
-Print Blow.
-Print Bhigh.
-
-Check set_digit.
-
-Fixpoint of_bvect (n:nat) : Bvector n -> int31 :=
- match n as n0 return Bvector n0 -> int31 with
- | O => fun _ => 0
- | S n' => fun v => set_digit (of_bvect n' (Bhigh n' v)) (of_Z (Z_of_nat n')) (Blow n' v)
- end.
-
-Axiom get_set_same : forall x p b,
-  ( (0 <= p) && (p < digits))%bool = true ->
-  get_digit (set_digit x p b) p = b.
-
-Axiom get_set_diff : forall x p p1 b1,
-  (p == p1)%bool = false ->
-  get_digit (set_digit x p1 b1) p = get_digit x p.
-
-Lemma toto : forall n v, to_bvect n (of_bvect n v) = v.
-Proof.
- induction n;simpl;intros.
- intros;symmetry;apply V0_eq.
-SearchAbout Vcons.
- rewrite (VSn_eq _ _ v);simpl.
- rewrite get_set_same.
- unfold Bcons.
- apply f_equal.
-Lemma tutu : forall n n' x b, (n <= n')%nat -> to_bvect n (set_digit x (of_Z (Z_of_nat n')) b) = to_bvect n x.
-Proof.
- induction n;simpl;intros;trivial.
- rewrite get_set_diff.
- apply f_equal.
- apply IHn;auto with arith.
- 
-
-
- SearchAbout Vhead.
-Print Blow.
- SearchAbout Vlow.
-SearchAbout Blow.
-
-
-
-Print Module Bvector.
-Check vec.
-
-Fixpoint mult_pow2 n z :=
- match n with
- | O => z
- | S n => Zdouble (mult_pow2 n z)
- end.
-
-Axiom lsl_spec : forall x p, to_Z2 (x << p) = (to_Z2 x * 2 ^ to_Z2 p) mod (2 ^ Z_of_nat size).
-
-Fixpoint Plor p1 p2 :=
- match p1, p2 with
- | xH, xH => 1%Z
- | xH, xO p2=> Zdouble_plus_one (Zpos p2)
- | xH, xI p2 => Zdouble_plus_one (Zpos p2)
- | xO p1, xH => Zdouble_plus_one (Zpos p1)
- | xI p2, xH => Zdouble_plus_one (Zpos p1)
- | xO p1, xO p2 => Zdouble (Plor p1 p2)
- | xI p1, xO p2 => Zdouble_plus_one (Plor p1 p2)
- | xO p1, xI p2 => Zdouble_plus_one (Plor p1 p2)
- | xI p1, xI p2 => Zdouble_plus_one (Plor p1 p2)
- end.
-
-Definition Zlor z1 z2 :=
- match z1, z2 with
- | Z0, _ => z2
- | _, Z0 => z1
- | Zpos p1, Zpos p2 => Zpos (Plor p1 p2)
- | Zneg p1, Zpos p2 => Zneg (Plor p1 p2)
- | Zpos p1, Zneg p2 => Zneg (Plor p1 p2)
- | Zneg p1, Zneg p2 => Zneg (Plor p1 p2)
- end.
-
-Axiom lor_spec : forall x y, to_Z2 (x lor y) = Zlor (to_Z2 x) (to_Z2 y).
-
-Lemma toto : forall x, to_Z2 ((x << 1) lor 1) = (2*to_Z2 x+1) mod (2 ^ Z_of_nat size).
-Proof.
- intros;rewrite lor_spec.
- rewrite lsl_spec.
- set (y:= to_Z2 1);change y with 1%Z;clear y.
- change (2 ^ 1)%Z with 2%Z.
- rewrite Zmult_comm.
-Lemma tutu : forall z, Zlor (2*z) 1 = (2*z + 1)%Z.
-Proof.
- destruct z;simpl.
-
-
-Lemma toto : forall x, to_Z2 size x = 1.
-intros.
- unfold to_Z2;simpl.
-*)
