theories/Numbers/Cyclic/Int31/Int31Properties.v
@@ -1,0 +1,966 @@
+Require Import Zgcd_alt.
+Require Import Bvector.
+Require Export Int31Axioms.
+
+
+Local Open Scope int31_scope.
+Local Open Scope Z_scope.
+(** Trivial lemmas without axiom *)
+
+Lemma wB_diff_0 : wB <> 0.
+Proof. compute;discriminate. Qed.
+
+Lemma wB_pos : 0 < wB.
+Proof. reflexivity. Qed.
+
+Lemma to_Z_0 : [|0|] = 0.
+Proof. reflexivity. Qed.
+
+Lemma to_Z_1 : [|1|] = 1.
+Proof. reflexivity. Qed.
+
+(** Bijection : int <-> Bvector size *)
+Lemma of_vect_inj : forall x y, of_vect x = of_vect y -> x = y.
+Proof.
+ intros.
+ rewrite <- (to_of_vect x), <- (to_of_vect y), H;trivial.
+Qed.
+
+Lemma of_to_vect : forall x, of_vect (to_vect x) = x.
+Proof.
+ intros;apply to_vect_inj.
+ rewrite to_of_vect;trivial.
+Qed.
+
+(** translation with Z *)
+Require Import Ndigits.
+
+Lemma Z_of_N_double : forall n, Z_of_N (Ndouble n) = Zdouble (Z_of_N n).
+Proof.
+ destruct n;simpl;trivial.
+Qed.
+
+Lemma Z_of_N_double_plus_one : forall n, Z_of_N (Ndouble_plus_one n) = Zdouble_plus_one (Z_of_N n).
+Proof.
+ destruct n;simpl;trivial.
+Qed.
+
+
+Lemma to_Z_to_vect : forall x, to_Z x = Z_of_N (Bv2N size (to_vect x)).
+Proof.
+ unfold to_Z, to_vect;generalize size.
+ induction n;simpl;intros;trivial.
+ destruct (is_even x);simpl.
+ rewrite Z_of_N_double, IHn;trivial.
+ rewrite Z_of_N_double_plus_one, IHn;trivial.
+Qed.
+
+Lemma of_vect_rec_false : forall n, of_vect_rec n (Bvect_false n) = 0%int31.
+Proof.
+ induction n;simpl;trivial.
+ unfold Bvect_false in IHn;rewrite IHn;trivial.
+Qed.
+
+
+Lemma of_Z_of_vect_pos : forall p, of_Z (Zpos p) = of_vect (N2Bv_gen size (Npos p)).
+Proof.
+ unfold of_Z, of_pos, of_vect;induction size;simpl;intros;trivial.
+ destruct p;simpl;try (rewrite IHn;trivial).
+ rewrite of_vect_rec_false;trivial.
+Qed.
+
+Lemma of_Z_of_vect_N : forall n, of_Z (Z_of_N n) = of_vect (N2Bv_gen size n).
+Proof.
+ destruct n;trivial.
+ apply of_Z_of_vect_pos.
+Qed.
+
+Lemma to_Z_bounded : forall x, 0 <= [|x|] < wB.
+Proof.
+ unfold to_Z, wB;induction size;intros.
+ simpl;auto with zarith.
+ rewrite inj_S;simpl;assert (W:= IHn (x >> 1)%int31).
+ rewrite Zpower_Zsucc;auto with zarith.
+ destruct (is_even x).
+ rewrite Zdouble_mult;auto with zarith.
+ rewrite Zdouble_plus_one_mult;auto with zarith.
+Qed.
+
+Lemma of_to_Z : forall x, of_Z ([|x|]) = x.
+Proof.
+ intros x; assert ([|x|] = Z_of_N (N_of_Z ([|x|]))).
+   destruct (to_Z_bounded x);destruct [|x|];trivial.
+   elim H;trivial.
+ rewrite H.
+ rewrite of_Z_of_vect_N.
+ rewrite to_Z_to_vect.
+ assert (forall n, N_of_Z (Z_of_N n) = n) by (destruct n;trivial).
+ rewrite H0, N2Bv_Bv2N, of_to_vect;trivial.
+Qed.
+
+Lemma is_even_lor1 : forall x, is_even ( x lor 1) = false.
+Proof.
+ intros.
+ unfold is_even, is_zero.
+ apply not_true_iff_false.
+ intros Heq;rewrite eqb_spec in Heq.
+ assert (W:= land_spec (x lor 1) 1).
+ rewrite Heq, lor_spec in W.
+ unfold to_vect in W;simpl in W.
+ injection W;clear W.
+ compute; do 30 intro;clear.
+ destruct (x land 1 == 0)%int31;discriminate.
+Qed.
+
+Lemma to_of_pos : forall p, [|of_pos p|] = Zpos p mod wB.
+Proof.
+ unfold to_Z, of_pos, wB;induction size;intros.
+ simpl;rewrite Zmod_1_r;trivial.
+ rewrite inj_S;simpl.
+ destruct p.
+ rewrite is_even_lor1.
+ (*** WARNING : *) 
+Admitted.
+
+Lemma to_of_Z : forall z, [| of_Z z |] = z mod wB.
+Proof.
+ destruct z;trivial; simpl of_Z.
+ rewrite to_of_pos;trivial.
+ unfold opp;rewrite sub_spec.
+ rewrite to_of_pos.
+ replace [|0|] with 0;trivial.
+ ring_simplify (0 - Zpos p mod wB).
+ change (Zneg p) with (- (Zpos p)).
+ destruct (Z_eq_dec (Zpos p mod wB) 0).
+ rewrite e. change (-0) with 0;rewrite Zmod_0_l.
+ rewrite Z_mod_zero_opp_full;trivial.
+ assert (W:= wB_diff_0); assert (W0:= wB_pos).
+ rewrite Z.mod_opp_l_nz;trivial.
+ rewrite Z.mod_opp_l_nz;trivial.
+ rewrite Zmod_small;trivial.
+ apply Z_mod_lt;auto with zarith.
+ rewrite Zmod_small;trivial.
+ apply Z_mod_lt;auto with zarith.
+Qed.
+
+Lemma to_Z_inj : forall x y, [|x|] = [|y|] -> x = y.
+Proof.
+ intros x y Heq.
+ rewrite <- (of_to_Z x), <- (of_to_Z y), Heq;trivial.
+Qed.
+
+(** leb *)
+(* TODO: move_this *)
+Lemma orb_true_iff : forall b1 b2, b1 || b2 = true <-> b1 = true \/ b2 = true.
+Proof.
+ split;intros;[apply orb_prop | apply orb_true_intro];trivial.
+Qed.
+
+Lemma to_Z_eq : forall x y, [|x|] = [|y|] <-> x = y.
+Proof.
+ split;intros;subst;trivial.
+ apply to_Z_inj;trivial.
+Qed.
+
+Lemma leb_ltb_eqb : forall x y, ((x <= y) = (x < y) || (x == y))%int31.
+Proof.
+ intros.
+ apply eq_true_iff_eq.
+ rewrite leb_spec, orb_true_iff, ltb_spec, eqb_spec, <- to_Z_eq;omega.
+Qed.
+
+(** Iterators *)
+
+Lemma foldi_gt : forall A f from to (a:A), 
+  (to < from)%int31 = true -> foldi f from to a = a.
+Proof.
+ intros;apply foldi_cont_gt;trivial.
+Qed.
+
+Lemma foldi_eq : forall A f from to (a:A),
+  from = to -> foldi f from to a = f from a.
+Proof.
+ intros;apply foldi_cont_eq;trivial.
+Qed.
+
+Lemma foldi_lt : forall A f from to (a:A), 
+  (from < to)%int31 = true -> foldi f from to a = foldi f (from + 1) to (f from a).
+Proof.
+ intros;apply foldi_cont_lt;trivial.
+Qed.
+
+Lemma fold_gt : forall A f from to (a:A), 
+  (to < from)%int31 = true -> fold f from to a = a.
+Proof.
+ intros;apply foldi_cont_gt;trivial.
+Qed.
+
+Lemma fold_eq : forall A f from to (a:A),
+  from = to -> fold f from to a = f a.
+Proof.
+ intros;apply foldi_cont_eq;trivial.
+Qed.
+
+Lemma fold_lt : forall A f from to (a:A), 
+  (from < to)%int31 = true -> fold f from to a = fold f (from + 1) to (f a).
+Proof.
+ intros;apply foldi_cont_lt;trivial.
+Qed.
+
+Lemma foldi_down_lt : forall A f from downto (a:A),
+  (from < downto)%int31 = true -> foldi_down f from downto a = a.
+Proof.
+ intros;apply foldi_down_cont_lt;trivial.
+Qed.
+
+Lemma foldi_down_eq : forall A f from downto (a:A),
+  from = downto -> foldi_down f from downto a = f from a.
+Proof.
+ intros;apply foldi_down_cont_eq;trivial.
+Qed.
+
+Lemma foldi_down_gt : forall A f from downto (a:A),
+  (downto < from)%int31 = true-> 
+  foldi_down f from downto a = 
+  foldi_down f (from-1) downto (f from a).
+Proof.
+ intros;apply foldi_down_cont_gt;trivial.
+Qed.
+
+Lemma fold_down_lt : forall A f from downto (a:A),
+  (from < downto)%int31 = true -> fold_down f from downto a = a.
+Proof.
+ intros;apply foldi_down_cont_lt;trivial.
+Qed.
+
+Lemma fold_down_eq : forall A f from downto (a:A),
+  from = downto -> fold_down f from downto a = f a.
+Proof.
+ intros;apply foldi_down_cont_eq;trivial.
+Qed.
+
+Lemma fold_down_gt : forall A f from downto (a:A),
+  (downto < from)%int31 = true-> 
+  fold_down f from downto a = 
+  fold_down f (from-1) downto (f a).
+Proof.
+ intros;apply foldi_down_cont_gt;trivial.
+Qed.
+
+(*
+Require Import Zwf.
+
+Lemma int31_ind : forall (P:int -> Type) x y,
+  P x ->
+  (forall z, 
+    ((x <= z) && (z < y))%int31 = true ->
+    (forall w, ((x <= w) && (w <= z))%int31 = true -> P w) ->
+    P (z + 1)%int31) ->
+  forall z , ((x <= z) && (z <= y))%int31 = true -> P z.
+Proof.
+ intros P x y Hx Hrec.
+ assert (forall Y, Acc (Zwf [|x|]) Y -> Y <= [|y|] -> 
+          (forall z, [|x|] <= [|z|] <= Y -> P z)).
+  intros Y Hacc;elim Hacc;intros Y0 _ Hrec0 Hley z (Hlex,HleY).
+ destruct (Z_le_lt_eq_dec _ _ HleY).
+ apply Hrec0 with [|z|].
+ red;omega. omega. omega.
+ destruct (Z_le_lt_eq_dec _ _ Hlex).
+
+
+ destruct (Zle_lt_or_eq _ _ HleY).
+
+ assert (W:= Zwf_well_founded [|x|] [|y|]).
+
+ elim W.
+ unfold Zwf.
+
+    (for
+((x <= z) && (z < y))%int31 = true -> P z) ->
+   (z < y)%int
+*)
+ 
+Lemma forallb_spec : forall f from to, 
+  forallb f from to = true ->
+  forall i, ((from <= i) && (i <= to))%int31 = true -> 
+  f i = true.
+Proof.
+ intros.
+(* Warning *)
+Admitted.
+
+Lemma existsb_spec : forall f from to,
+  existsb f from to = true ->
+  exists i, ((from <= i) && (i <= to))%int31 = true -> f i = true.
+Proof.
+ intros.
+(* Warning *)
+Admitted.
+
+(** Comparison *)
+
+Lemma compare_spec :
+  forall x y, compare x y = ([|x|] ?= [|y|]).
+Proof.
+ intros;rewrite compare_def_spec;unfold compare_def.
+ case_eq (x < y)%int31;intros Heq.
+ rewrite ltb_spec in Heq.
+ red in Heq;rewrite Heq;trivial.
+ rewrite <- not_true_iff_false, ltb_spec in Heq.
+ case_eq (x == y)%int31;intros Heq1.
+ rewrite eqb_spec in Heq1;rewrite Heq1, Zcompare_refl;trivial.
+ rewrite <- not_true_iff_false, eqb_spec in Heq1.
+ symmetry;change ([|x|] > [|y|]);rewrite <- to_Z_eq in Heq1;omega.
+Qed.
+
+
+Lemma is_zero_spec : forall x : int, is_zero x = true <-> x = 0%int31.
+Proof.
+ unfold is_zero;intros;apply eqb_spec.
+Qed.
+
+(* TODO : remove this axiom *)
+Lemma is_even_spec : forall x,
+      if is_even x then [|x|] mod 2 = 0 else [|x|] mod 2 = 1.
+Proof.
+ unfold is_even;intros.
+Admitted.
+
+
+(** Addition *)
+
+Lemma addc_spec  : forall x y, [+|x +c y|] = [|x|] + [|y|].
+Proof.
+ intros;rewrite addc_def_spec;unfold addc_def.
+ assert (W1 := to_Z_bounded x); assert (W2 := to_Z_bounded y).
+ case_eq ((x + y < x)%int31).
+ rewrite ltb_spec;intros.
+ change (wB + [|x+y|] = [|x|] + [|y|]).
+ rewrite add_spec in H |- *.
+ assert ([|x|] + [|y|] >= wB).
+  destruct (Z_lt_ge_dec ([|x|] + [|y|]) wB);auto with zarith.
+  elimtype False;rewrite Zmod_small in H;auto with zarith.
+ assert (([|x|] + [|y|]) mod wB = [|x|] + [|y|] - wB).
+  symmetry;apply Zmod_unique with 1;auto with zarith.
+ rewrite H1;ring.
+ rewrite <- not_true_iff_false, ltb_spec;intros.
+ change ([|x+y|] = [|x|] + [|y|]).
+ rewrite add_spec in *.
+ assert ([|x|] + [|y|] < wB).
+  destruct (Z_lt_ge_dec ([|x|] + [|y|]) wB);auto with zarith.
+  assert (([|x|] + [|y|]) mod wB = [|x|] + [|y|] - wB).
+  symmetry;apply Zmod_unique with 1;auto with zarith.
+  elim H;omega.
+ rewrite Zmod_small;auto with zarith.
+Qed.
+
+Lemma succc_spec : forall x, [+|succc x|] = [|x|] + 1.
+Proof. intros; apply addc_spec. Qed.
+
+Lemma addcarry_spec : forall x y, [|addcarry x y|] = ([|x|] + [|y|] + 1) mod wB.
+Proof.
+ unfold addcarry;intros.
+ rewrite add_spec,add_spec,Zplus_mod_idemp_l;trivial.
+Qed.
+
+Lemma addcarryc_spec : forall x y, [+|addcarryc x y|] = [|x|] + [|y|] + 1.
+Proof.
+ intros;rewrite addcarryc_def_spec;unfold addcarryc_def.
+ assert (W1 := to_Z_bounded x); assert (W2 := to_Z_bounded y).
+ case_eq ((addcarry x y <= x)%int31).
+ rewrite leb_spec;intros.
+ change (wB + [|(addcarry x y)|] = [|x|] + [|y|] + 1).
+ rewrite addcarry_spec in H |- *.
+ assert ([|x|] + [|y|] + 1 >= wB).
+  destruct (Z_lt_ge_dec ([|x|] + [|y|] + 1) wB);auto with zarith.
+  elimtype False;rewrite Zmod_small in H;auto with zarith.
+ assert (([|x|] + [|y|] + 1) mod wB = [|x|] + [|y|] + 1 - wB).
+  symmetry;apply Zmod_unique with 1;auto with zarith.
+ rewrite H1;ring.
+ rewrite <- not_true_iff_false, leb_spec;intros.
+ change ([|addcarry x y|] = [|x|] + [|y|] + 1).
+ rewrite addcarry_spec in *.
+ assert ([|x|] + [|y|] + 1 < wB).
+  destruct (Z_lt_ge_dec ([|x|] + [|y|] + 1) wB);auto with zarith.
+  assert (([|x|] + [|y|] + 1) mod wB = [|x|] + [|y|] + 1 - wB).
+  symmetry;apply Zmod_unique with 1;auto with zarith.
+  elim H;omega.
+ rewrite Zmod_small;auto with zarith.
+Qed.
+
+Lemma succ_spec : forall x, [|succ x|] = ([|x|] + 1) mod wB.
+Proof. intros; apply add_spec. Qed.
+
+(** Subtraction *)
+Lemma subc_spec : forall x y, [-|x -c y|] = [|x|] - [|y|].
+Proof.
+ intros;rewrite subc_def_spec;unfold subc_def.
+ assert (W1 := to_Z_bounded x); assert (W2 := to_Z_bounded y).
+ case_eq (y <= x)%int31.
+ rewrite leb_spec;intros.
+ change ([|x - y|] = [|x|] - [|y|]).
+ rewrite sub_spec.
+ rewrite Zmod_small;auto with zarith.
+ rewrite <- not_true_iff_false, leb_spec;intros.
+ change (-wB + [|x - y|] = [|x|] - [|y|]).
+ rewrite sub_spec.
+ assert (([|x|] - [|y|]) mod wB = [|x|] - [|y|] + wB).
+  symmetry;apply Zmod_unique with (-1);auto with zarith.
+ rewrite H0;ring.
+Qed.
+
+Lemma subcarry_spec :
+   forall x y, [|subcarry x y|] = ([|x|] - [|y|] - 1) mod wB.
+Proof. 
+ unfold subcarry; intros.
+ rewrite sub_spec,sub_spec,Zminus_mod_idemp_l;trivial.
+Qed.
+
+Lemma subcarryc_spec : forall x y, [-|subcarryc x y|] = [|x|] - [|y|] - 1.
+ intros;rewrite subcarryc_def_spec;unfold subcarryc_def.
+ assert (W1 := to_Z_bounded x); assert (W2 := to_Z_bounded y).
+ fold (subcarry x y).
+ case_eq (y < x)%int31.
+ rewrite ltb_spec;intros.
+ change ([|subcarry x y|] = [|x|] - [|y|] - 1).
+ rewrite subcarry_spec.
+ rewrite Zmod_small;auto with zarith.
+ rewrite <- not_true_iff_false, ltb_spec;intros.
+ change (-wB + [|subcarry x y|] = [|x|] - [|y|] - 1).
+ rewrite subcarry_spec.
+ assert (([|x|] - [|y|] - 1) mod wB = [|x|] - [|y|] - 1 + wB).
+  symmetry;apply Zmod_unique with (-1);auto with zarith.
+ rewrite H0;ring.
+Qed.
+
+Lemma oppc_spec : forall x : int, [-|oppc x|] = - [|x|].
+Proof.
+ unfold oppc;intros;rewrite subc_spec, to_Z_0;trivial.
+Qed.
+
+Lemma opp_spec : forall x : int, [|- x|] = - [|x|] mod wB.
+Proof.
+ unfold opp;intros;rewrite sub_spec, to_Z_0;trivial.
+Qed.
+
+Lemma oppcarry_spec : forall x, [|oppcarry x|] = wB - [|x|] - 1.
+Proof.
+ unfold oppcarry;intros.
+ rewrite sub_spec.
+ change [|max_int|] with (wB - 1).
+ rewrite <- Zminus_plus_distr, Zplus_comm, Zminus_plus_distr.
+ apply Zmod_small.
+ generalize (to_Z_bounded x);auto with zarith.
+Qed.
+
+Lemma predc_spec : forall x, [-|predc x|] = [|x|] - 1.
+Proof. intros; apply subc_spec. Qed.
+
+Lemma pred_spec : forall x, [|pred x|] = ([|x|] - 1) mod wB.
+Proof. intros; apply sub_spec. Qed.
+
+Lemma diveucl_spec : 
+  forall x y, 
+    let (q,r) := diveucl x y in
+    ([|q|],[|r|]) = Zdiv_eucl [|x|] [|y|].
+Proof.
+ intros;rewrite diveucl_def_spec.
+ unfold diveucl_def;rewrite div_spec, mod_spec.
+ unfold Zdiv, Zmod;destruct (Zdiv_eucl [|x|] [|y|]);trivial.
+Qed.
+
+(* Sqrt *)
+
+ (* Direct transcription of an old proof
+     of a fortran program in boyer-moore *)
+
+Lemma quotient_by_2 a: a - 1 <= (a/2) + (a/2).
+Proof.
+ case (Z_mod_lt a 2); auto with zarith.
+ intros H1; rewrite Zmod_eq_full; auto with zarith.
+Qed.
+
+Lemma sqrt_main_trick j k: 0 <= j -> 0 <= k ->
+   (j * k) + j <= ((j + k)/2 + 1)  ^ 2.
+Proof.
+ intros Hj; generalize Hj k; pattern j; apply natlike_ind;
+   auto; clear k j Hj.
+ intros _ k Hk; repeat rewrite Zplus_0_l.
+ apply  Zmult_le_0_compat; generalize (Z_div_pos k 2); auto with zarith.
+ intros j Hj Hrec _ k Hk; pattern k; apply natlike_ind; auto; clear k Hk.
+ rewrite Zmult_0_r, Zplus_0_r, Zplus_0_l.
+ generalize (sqr_pos (Zsucc j / 2)) (quotient_by_2 (Zsucc j));
+   unfold Zsucc.
+ rewrite Zpower_2, Zmult_plus_distr_l; repeat rewrite Zmult_plus_distr_r.
+ auto with zarith.
+ intros k Hk _.
+ replace ((Zsucc j + Zsucc k) / 2) with ((j + k)/2 + 1).
+ generalize (Hrec Hj k Hk) (quotient_by_2 (j + k)).
+ unfold Zsucc; repeat rewrite Zpower_2;
+   repeat rewrite Zmult_plus_distr_l; repeat rewrite Zmult_plus_distr_r.
+ repeat rewrite Zmult_1_l; repeat rewrite Zmult_1_r.
+ auto with zarith.
+ rewrite Zplus_comm, <- Z_div_plus_full_l; auto with zarith.
+ apply f_equal2 with (f := Zdiv); auto with zarith.
+Qed.
+
+Lemma sqrt_main i j: 0 <= i -> 0 < j -> i < ((j + (i/j))/2 + 1) ^ 2.
+Proof.
+ intros Hi Hj.
+ assert (Hij: 0 <= i/j) by (apply Z_div_pos; auto with zarith).
+ apply Zlt_le_trans with (2 := sqrt_main_trick _ _ (Zlt_le_weak _ _ Hj) Hij).
+ pattern i at 1; rewrite (Z_div_mod_eq i j); case (Z_mod_lt i j); auto with zarith.
+Qed.
+
+Lemma sqrt_init i: 1 < i -> i < (i/2 + 1) ^ 2.
+Proof.
+ intros Hi.
+ assert (H1: 0 <= i - 2) by auto with zarith.
+ assert (H2: 1 <= (i / 2) ^ 2); auto with zarith.
+   replace i with (1* 2 + (i - 2)); auto with zarith.
+   rewrite Zpower_2, Z_div_plus_full_l; auto with zarith.
+   generalize (sqr_pos ((i - 2)/ 2)) (Z_div_pos (i - 2) 2).
+   rewrite Zmult_plus_distr_l; repeat rewrite Zmult_plus_distr_r.
+   auto with zarith.
+ generalize (quotient_by_2 i).
+ rewrite Zpower_2 in H2 |- *;
+   repeat (rewrite Zmult_plus_distr_l ||
+           rewrite Zmult_plus_distr_r ||
+           rewrite Zmult_1_l || rewrite Zmult_1_r).
+   auto with zarith.
+Qed.
+
+Lemma sqrt_test_true i j: 0 <= i -> 0 < j -> i/j >= j -> j ^ 2 <= i.
+Proof.
+ intros Hi Hj Hd; rewrite Zpower_2.
+ apply Zle_trans with (j * (i/j)); auto with zarith.
+ apply Z_mult_div_ge; auto with zarith.
+Qed.
+
+Lemma sqrt_test_false i j: 0 <= i -> 0 < j -> i/j < j ->  (j + (i/j))/2 < j.
+Proof.
+ intros Hi Hj H; case (Zle_or_lt j ((j + (i/j))/2)); auto.
+ intros H1; contradict H; apply Zle_not_lt.
+ assert (2 * j <= j + (i/j)); auto with zarith.
+ apply Zle_trans with (2 * ((j + (i/j))/2)); auto with zarith.
+ apply Z_mult_div_ge; auto with zarith.
+Qed.
+
+Lemma sqrt_step_correct rec i j:
+  0 < [|i|] -> 0 < [|j|] -> [|i|] < ([|j|] + 1) ^ 2 ->
+   2 * [|j|] < wB ->
+  (forall j1 : int,
+    0 < [|j1|] < [|j|] -> [|i|] < ([|j1|] + 1) ^ 2 ->
+    [|rec i j1|] ^ 2 <= [|i|] < ([|rec i j1|] + 1) ^ 2) ->
+  [|sqrt_step rec i j|] ^ 2 <= [|i|] < ([|sqrt_step rec i j|] + 1) ^ 2.
+Proof.
+ assert (Hp2: 0 < [|2|]) by exact (refl_equal Lt).
+ intros Hi Hj Hij H31 Hrec.
+ unfold sqrt_step.
+ case_eq ((i / j < j)%int31);[ | rewrite <- Bool.not_true_iff_false];
+  rewrite ltb_spec, div_spec;intros.
+ assert ([| j + i / j|] = [|j|] + [|i|]/[|j|]).
+   rewrite add_spec, Zmod_small;rewrite div_spec;auto with zarith.
+ apply Hrec;rewrite lsr_spec, H0, to_Z_1;change (2^1) with 2.
+ split; [ | apply sqrt_test_false;auto with zarith].
+ replace ([|j|] + [|i|]/[|j|]) with
+        (1 * 2 + (([|j|] - 2) + [|i|] / [|j|]));[ | ring].
+ rewrite Z_div_plus_full_l; auto with zarith.
+ assert (0 <= [|i|]/ [|j|]) by (apply Z_div_pos; auto with zarith).
+ assert (0 <= ([|j|] - 2 + [|i|] / [|j|]) / 2) ; auto with zarith.
+ case (Zle_lt_or_eq 1 [|j|]); auto with zarith; intros Hj1.
+ rewrite <- Hj1, Zdiv_1_r.
+ assert (0 <= ([|i|] - 1) /2)%Z;[ |apply Z_div_pos]; auto with zarith.
+ apply sqrt_main;auto with zarith.
+ split;[apply sqrt_test_true | ];auto with zarith.
+Qed.
+ 
+Lemma iter_sqrt_correct n rec i j: 0 < [|i|] -> 0 < [|j|] ->
+  [|i|] < ([|j|] + 1) ^ 2 -> 2 * [|j|] < wB ->
+  (forall j1, 0 < [|j1|] -> 2^(Z_of_nat n) + [|j1|] <= [|j|] ->
+      [|i|] < ([|j1|] + 1) ^ 2 -> 2 * [|j1|] < wB ->
+       [|rec i j1|] ^ 2 <= [|i|] < ([|rec i j1|] + 1) ^ 2) ->
+  [|iter_sqrt n rec i j|] ^ 2 <= [|i|] < ([|iter_sqrt n rec i j|] + 1) ^ 2.
+Proof.
+ revert rec i j; elim n; unfold iter_sqrt; fold iter_sqrt; clear n.
+ intros rec i j Hi Hj Hij H31 Hrec; apply sqrt_step_correct; auto with zarith.
+ intros; apply Hrec; auto with zarith.
+ rewrite Zpower_0_r; auto with zarith.
+ intros n Hrec rec i j Hi Hj Hij H31 HHrec.
+ apply sqrt_step_correct; auto.
+ intros j1 Hj1  Hjp1; apply Hrec; auto with zarith.
+ intros j2 Hj2 H2j2 Hjp2 Hj31; apply Hrec; auto with zarith.
+ intros j3 Hj3 Hpj3.
+ apply HHrec; auto.
+ rewrite inj_S, Zpower_Zsucc.
+ apply Zle_trans with (2 ^Z_of_nat n + [|j2|]); auto with zarith.
+ apply Zle_0_nat.
+Qed.
+
+Lemma sqrt_spec : forall x,
+       [|sqrt x|] ^ 2 <= [|x|] < ([|sqrt x|] + 1) ^ 2.
+Proof.
+ intros i; unfold sqrt.
+ rewrite compare_spec. case Zcompare_spec; rewrite to_Z_1;
+   intros Hi; auto with zarith.
+ repeat rewrite Zpower_2; auto with zarith.
+ apply iter_sqrt_correct; auto with zarith;
+  rewrite lsr_spec, to_Z_1; change (2^1) with 2;  auto with zarith.
+  replace ([|i|]) with (1 * 2 + ([|i|] - 2))%Z; try ring.
+  assert (0 <= ([|i|] - 2)/2)%Z by (apply Z_div_pos; auto with zarith).
+  rewrite Z_div_plus_full_l; auto with zarith.
+  apply sqrt_init; auto.
+  assert (W:= Z_mult_div_ge [|i|] 2);assert (W':= to_Z_bounded i);auto with zarith.
+  intros j2 H1 H2; contradict H2; apply Zlt_not_le.
+  fold wB;assert (W:=to_Z_bounded i).
+  apply Zle_lt_trans with ([|i|]); auto with zarith.
+  assert (0 <= [|i|]/2)%Z by (apply Z_div_pos; auto with zarith).
+  apply Zle_trans with (2 * ([|i|]/2)); auto with zarith.
+  apply Z_mult_div_ge; auto with zarith.
+ case (to_Z_bounded i); repeat rewrite Zpower_2; auto with zarith.
+Qed.
+
+Lemma sqrt2_step_def rec ih il j:
+   sqrt2_step rec ih il j =
+   if (ih < j)%int31 then
+    let quo := fst (diveucl_21 ih il j) in
+    if (quo < j)%int31 then
+     let m :=
+      match j +c quo with
+      | C0 m1 => m1 >> 1
+      | C1 m1 => (m1 >> 1 + 30)%int31
+      end in
+     rec ih il m
+    else j
+   else j.
+Proof.
+ unfold sqrt2_step; case diveucl_21; intros;simpl.
+ case (j +c i);trivial.
+Qed.
+
+Lemma sqrt2_lower_bound ih il j:
+   [|| WW ih il||]  < ([|j|] + 1) ^ 2 -> [|ih|] <= [|j|].
+Proof.
+ intros H1.
+ case (to_Z_bounded j); intros Hbj _.
+ case (to_Z_bounded il); intros Hbil _.
+ case (to_Z_bounded ih); intros Hbih Hbih1.
+ assert (([|ih|] < [|j|] + 1)%Z); auto with zarith.
+ apply Zlt_square_simpl; auto with zarith.
+ simpl zn2z_to_Z in H1.
+ repeat rewrite <-Zpower_2; apply Zle_lt_trans with (2 := H1).
+ apply Zle_trans with ([|ih|] * wB)%Z;try rewrite Zpower_2; auto with zarith.
+Qed.
+
+Lemma div2_phi ih il j: 
+  [|fst (diveucl_21 ih il j)|] = [|| WW ih il||] /[|j|].
+Proof.
+ generalize (diveucl_21_spec ih il j).
+ case diveucl_21; intros q r Heq.
+ simpl zn2z_to_Z;unfold Zdiv;rewrite <- Heq;trivial.
+Qed.
+
+Lemma zn2z_to_Z_pos ih il : 0 <= [||WW ih il||].
+Proof.
+ simpl zn2z_to_Z;destruct (to_Z_bounded ih);destruct (to_Z_bounded il);auto with zarith.
+Qed.
+
+
+Lemma sqrt2_step_correct rec ih il j:
+  2 ^ (Z_of_nat (size - 2)) <= [|ih|] -> 
+  0 < [|j|] -> [|| WW ih il||] < ([|j|] + 1) ^ 2 ->
+  (forall j1, 0 < [|j1|] < [|j|] ->  [|| WW ih il||] < ([|j1|] + 1) ^ 2 ->
+     [|rec ih il j1|] ^ 2 <= [||WW ih il||] < ([|rec ih il j1|] + 1) ^ 2) ->
+  [|sqrt2_step rec ih il j|] ^ 2 <= [||WW ih il ||]
+      < ([|sqrt2_step rec ih il j|] + 1) ^  2.
+(*** WARNING : TODO *)
+Admitted.
+(*
+Proof.
+ assert (Hp2: (0 < [|2|])%Z) by exact (refl_equal Lt).
+ intros Hih Hj Hij Hrec; rewrite sqrt2_step_def.
+ assert (H1: ([|ih|] <= [|j|])%Z) by (apply sqrt2_lower_bound with il; auto).
+ case (to_Z_bounded ih); intros Hih1 _.
+ case (to_Z_bounded il); intros Hil1 _.
+ case (to_Z_bounded j); intros _ Hj1.
+ assert (Hp3: (0 < [||WW ih il||])).
+  simpl zn2z_to_Z;apply Zlt_le_trans with ([|ih|] * wB)%Z; auto with zarith.
+  apply Zmult_lt_0_compat; auto with zarith.
+  apply Zlt_le_trans with (2:= Hih); auto with zarith.
+ cbv zeta.
+ case_eq (ih < j)%int31;intros Heq.
+ rewrite ltb_spec in Heq.
+ case_eq (fst (diveucl_21 ih il j) < j)%int31;intros Heq0.
+ rewrite ltb_spec in Heq0.
+ assert ([|match j +c fst (diveucl_21 ih il j) with
+           | C0 m1 => m1 >> 1
+           | C1 m1 => (m1 >> 1 + 30)%int31
+           end|] = ([|j|] + ([||WW ih il||])/([|j|]))/2).
+  generalize (addc_spec j (fst (diveucl_21 ih il j)));
+  case addc;unfold interp_carry;rewrite div2_phi;simpl zn2z_to_Z.
+  intros i H;rewrite lsr_spec, H;trivial.
+  intros i H;rewrite <- H.
+(*** Warning : TODO *)
+  admit.
+ apply Hrec;rewrite H.
+  (*** Warning : TODO *)
+  admit.
+  admit.
+ split;auto.
+ apply sqrt_test_true; auto.
+ apply zn2z_to_Z_pos.
+ rewrite <- not_true_iff_false, ltb_spec in Heq0.
+ assert (W:= diveucl_21_spec ih il j).
+ destruct (diveucl_21 ih il j).
+ unfold Zdiv;simpl zn2z_to_Z;rewrite <- W;simpl in Heq0;auto with zarith.
+ split;auto.
+ apply sqrt_test_true; auto.
+ apply zn2z_to_Z_pos.
+ rewrite <- not_true_iff_false, ltb_spec in Heq.
+ simpl zn2z_to_Z.
+ (*** Warning : TODO *)
+ admit.
+Qed.
+*)
+(*
+ Lemma iter312_sqrt_correct n rec ih il j:
+  2^29 <= [|ih|] ->  0 < [|j|] -> phi2 ih il < ([|j|] + 1) ^ 2 ->
+  (forall j1, 0 < [|j1|] -> 2^(Z_of_nat n) + [|j1|] <= [|j|] ->
+      phi2 ih il < ([|j1|] + 1) ^ 2 ->
+       [|rec ih il j1|] ^ 2 <= phi2 ih il < ([|rec ih il j1|] + 1) ^ 2)  ->
+  [|iter312_sqrt n rec ih il j|] ^ 2 <= phi2 ih il
+      < ([|iter312_sqrt n rec ih il j|] + 1) ^ 2.
+ Proof.
+ revert rec ih il j; elim n; unfold iter312_sqrt; fold iter312_sqrt; clear n.
+ intros rec ih il j Hi Hj Hij Hrec; apply sqrt312_step_correct; auto with zarith.
+ intros; apply Hrec; auto with zarith.
+ rewrite Zpower_0_r; auto with zarith.
+ intros n Hrec rec ih il j Hi Hj Hij HHrec.
+ apply sqrt312_step_correct; auto.
+ intros j1 Hj1  Hjp1; apply Hrec; auto with zarith.
+ intros j2 Hj2 H2j2 Hjp2; apply Hrec; auto with zarith.
+ intros j3 Hj3 Hpj3.
+ apply HHrec; auto.
+ rewrite inj_S, Zpower_Zsucc.
+ apply Zle_trans with (2 ^Z_of_nat n + [|j2|])%Z; auto with zarith.
+ apply Zle_0_nat.
+ Qed.
+*)
+Lemma sqrt2_spec : forall x y,
+       wB/ 4 <= [|x|] ->
+       let (s,r) := sqrt2 x y in
+          [||WW x y||] = [|s|] ^ 2 + [+|r|] /\
+          [+|r|] <= 2 * [|s|].
+(* WARNING TODO *)
+Admitted.
+(*
+ Proof.
+ intros ih il Hih; unfold sqrt312.
+ change [||WW ih il||] with (phi2 ih il).
+ assert (Hbin: forall s, s * s + 2* s + 1 = (s + 1) ^ 2) by
+  (intros s; ring).
+ assert (Hb: 0 <= base) by (red; intros HH; discriminate).
+ assert (Hi2: phi2 ih il < (phi Tn + 1) ^ 2).
+   change ((phi Tn + 1) ^ 2) with (2^62).
+  apply Zle_lt_trans with ((2^31 -1) * base + (2^31 - 1)); auto with zarith.
+  2: simpl; unfold Zpower_pos; simpl; auto with zarith.
+  case (phi_bounded ih); case (phi_bounded il); intros H1 H2 H3 H4.
+  unfold base, Zpower, Zpower_pos in H2,H4; simpl in H2,H4.
+  unfold phi2,Zpower, Zpower_pos; simpl iter_pos; auto with zarith.
+ case (iter312_sqrt_correct 31 (fun _ _ j => j) ih il Tn); auto with zarith.
+ change [|Tn|] with 2147483647; auto with zarith.
+ intros j1 _ HH; contradict HH.
+ apply Zlt_not_le.
+ change [|Tn|] with 2147483647; auto with zarith.
+ change (2 ^ Z_of_nat 31) with 2147483648; auto with zarith.
+ case (phi_bounded j1); auto with zarith.
+ set (s := iter312_sqrt 31 (fun _ _ j : int31 => j) ih il Tn).
+ intros Hs1 Hs2.
+ generalize (spec_mul_c s s); case mul31c.
+ simpl zn2z_to_Z; intros HH.
+ assert ([|s|] = 0).
+ case (Zmult_integral _ _ (sym_equal HH)); auto.
+ contradict Hs2; apply Zle_not_lt; rewrite H.
+ change ((0 + 1) ^ 2) with 1.
+ apply Zle_trans with (2 ^ Z_of_nat size / 4 * base).
+ simpl; auto with zarith.
+ apply Zle_trans with ([|ih|] * base); auto with zarith.
+ unfold phi2; case (phi_bounded il); auto with zarith.
+ intros ih1 il1.
+ change [||WW ih1 il1||] with (phi2 ih1 il1).
+ intros Hihl1.
+ generalize (spec_sub_c il il1).
+ case sub31c; intros il2 Hil2.
+ simpl interp_carry in Hil2.
+ rewrite spec_compare; case Zcompare_spec.
+ unfold interp_carry.
+ intros H1; split.
+ rewrite Zpower_2, <- Hihl1.
+ unfold phi2; ring[Hil2 H1].
+ replace [|il2|] with (phi2 ih il - phi2 ih1 il1).
+ rewrite Hihl1.
+ rewrite <-Hbin in Hs2; auto with zarith.
+ unfold phi2; rewrite H1, Hil2; ring.
+ unfold interp_carry.
+ intros H1; contradict Hs1.
+ apply Zlt_not_le; rewrite Zpower_2, <-Hihl1.
+ unfold phi2.
+ case (phi_bounded il); intros _ H2.
+ apply Zlt_le_trans with (([|ih|] + 1) * base + 0).
+ rewrite Zmult_plus_distr_l, Zplus_0_r; auto with zarith.
+ case (phi_bounded il1); intros H3 _.
+ apply Zplus_le_compat; auto with zarith.
+ unfold interp_carry; change (1 * 2 ^ Z_of_nat size) with base.
+ rewrite Zpower_2, <- Hihl1, Hil2.
+ intros H1.
+ case (Zle_lt_or_eq ([|ih1|] + 1) ([|ih|])); auto with zarith.
+ intros H2; contradict Hs2; apply Zle_not_lt.
+ replace (([|s|] + 1) ^ 2) with (phi2 ih1 il1 + 2 * [|s|] + 1).
+ unfold phi2.
+ case (phi_bounded il); intros Hpil _.
+ assert (Hl1l: [|il1|] <= [|il|]).
+  case (phi_bounded il2); rewrite Hil2; auto with zarith.
+ assert ([|ih1|] * base + 2 * [|s|] + 1 <= [|ih|] * base); auto with zarith.
+ case (phi_bounded s);  change (2 ^ Z_of_nat size) with base; intros _ Hps.
+ case (phi_bounded ih1); intros Hpih1 _; auto with zarith.
+ apply Zle_trans with (([|ih1|] + 2) * base); auto with zarith.
+ rewrite Zmult_plus_distr_l.
+ assert (2 * [|s|] + 1 <= 2 * base); auto with zarith.
+ rewrite Hihl1, Hbin; auto.
+ intros H2; split.
+ unfold phi2; rewrite <- H2; ring.
+ replace (base + ([|il|] - [|il1|])) with (phi2 ih il - ([|s|] * [|s|])).
+ rewrite <-Hbin in Hs2; auto with zarith.
+ rewrite <- Hihl1; unfold phi2; rewrite <- H2; ring.
+ unfold interp_carry in Hil2 |- *.
+ unfold interp_carry; change (1 * 2 ^ Z_of_nat size) with base.
+ assert (Hsih: [|ih - 1|] = [|ih|] - 1).
+  rewrite spec_sub, Zmod_small; auto; change [|1|] with 1.
+  case (phi_bounded ih); intros H1 H2.
+  generalize Hih; change (2 ^ Z_of_nat size / 4) with 536870912.
+  split; auto with zarith.
+ rewrite spec_compare; case Zcompare_spec.
+ rewrite Hsih.
+ intros H1; split.
+ rewrite Zpower_2, <- Hihl1.
+ unfold phi2; rewrite <-H1.
+ apply trans_equal with ([|ih|] * base + [|il1|] + ([|il|] - [|il1|])).
+ ring.
+ rewrite <-Hil2.
+ change (2 ^ Z_of_nat size) with base; ring.
+ replace [|il2|] with (phi2 ih il - phi2 ih1 il1).
+ rewrite Hihl1.
+ rewrite <-Hbin in Hs2; auto with zarith.
+ unfold phi2.
+ rewrite <-H1.
+ ring_simplify.
+ apply trans_equal with (base + ([|il|] - [|il1|])).
+ ring.
+ rewrite <-Hil2.
+ change (2 ^ Z_of_nat size) with base; ring.
+ rewrite Hsih; intros H1.
+ assert (He: [|ih|] = [|ih1|]).
+   apply Zle_antisym; auto with zarith.
+   case (Zle_or_lt [|ih1|] [|ih|]); auto; intros H2.
+   contradict Hs1; apply Zlt_not_le; rewrite Zpower_2, <-Hihl1.
+  unfold phi2.
+  case (phi_bounded il); change (2 ^ Z_of_nat size) with base;
+    intros _ Hpil1.
+  apply Zlt_le_trans with (([|ih|] + 1) * base).
+  rewrite Zmult_plus_distr_l, Zmult_1_l; auto with zarith.
+  case (phi_bounded il1); intros Hpil2 _.
+  apply Zle_trans with (([|ih1|]) * base); auto with zarith.
+ rewrite Zpower_2, <-Hihl1; unfold phi2; rewrite <-He.
+ contradict Hs1; apply Zlt_not_le; rewrite Zpower_2, <-Hihl1.
+ unfold phi2; rewrite He.
+ assert (phi il - phi il1 < 0); auto with zarith.
+ rewrite <-Hil2.
+ case (phi_bounded il2); auto with zarith.
+ intros H1.
+ rewrite Zpower_2, <-Hihl1.
+ case (Zle_lt_or_eq ([|ih1|] + 2) [|ih|]); auto with zarith.
+ intros H2; contradict Hs2; apply Zle_not_lt.
+ replace (([|s|] + 1) ^ 2) with (phi2 ih1 il1 + 2 * [|s|] + 1).
+ unfold phi2.
+ assert ([|ih1|] * base + 2 * phi s + 1 <= [|ih|] * base + ([|il|] - [|il1|]));
+  auto with zarith.
+ rewrite <-Hil2.
+ change (-1 * 2 ^ Z_of_nat size) with (-base).
+ case (phi_bounded il2); intros Hpil2 _.
+ apply Zle_trans with ([|ih|] * base + - base); auto with zarith.
+ case (phi_bounded s);  change (2 ^ Z_of_nat size) with base; intros _ Hps.
+ assert (2 * [|s|] + 1 <= 2 * base); auto with zarith.
+ apply Zle_trans with ([|ih1|] * base + 2 * base); auto with zarith.
+ assert (Hi: ([|ih1|] + 3) * base <= [|ih|] * base); auto with zarith.
+ rewrite Zmult_plus_distr_l in Hi; auto with zarith.
+ rewrite Hihl1, Hbin; auto.
+ intros H2; unfold phi2; rewrite <-H2.
+ split.
+ replace [|il|] with (([|il|] - [|il1|]) + [|il1|]); try ring.
+ rewrite <-Hil2.
+ change (-1 * 2 ^ Z_of_nat size) with (-base); ring.
+ replace (base + [|il2|]) with (phi2 ih il - phi2 ih1 il1).
+ rewrite Hihl1.
+ rewrite <-Hbin in Hs2; auto with zarith.
+ unfold phi2; rewrite <-H2.
+ replace [|il|] with (([|il|] - [|il1|]) + [|il1|]); try ring.
+ rewrite <-Hil2.
+ change (-1 * 2 ^ Z_of_nat size) with (-base); ring.
+Qed.
+*)
+
+Lemma to_Z_gcd : forall i j,
+  [|gcd i j|] = Zgcdn (2*size) [|j|] [|i|].
+Proof.
+ unfold gcd.
+ induction (2*size)%nat; intros.
+ reflexivity.
+ simpl.
+ generalize (to_Z_bounded j)(to_Z_bounded i); intros.
+ case_eq (j == 0)%int31.
+ rewrite eqb_spec;intros H1;rewrite H1.
+ replace [|0|] with 0;trivial;rewrite Z.abs_eq;auto with zarith.
+ rewrite <- not_true_iff_false, eqb_spec;intros.
+ case_eq [|j|]; intros.
+ elim H1;apply to_Z_inj;assumption.
+ rewrite IHn, <- H2, mod_spec;trivial.
+ rewrite H2 in H;destruct H as (H, _);elim H;trivial.
+Qed.
+
+Lemma gcd_spec : forall a b, Zis_gcd [|a|] [|b|] [|gcd a b|].
+Proof.
+ intros.
+ rewrite to_Z_gcd.
+ apply Zis_gcd_sym.
+ apply Zgcdn_is_gcd.
+ unfold Zgcd_bound.
+ generalize (to_Z_bounded b).
+ destruct [|b|].
+ unfold size; auto with zarith.
+ intros (_,H).
+ cut (Psize p <= size)%nat; [ omega | rewrite <- Zpower2_Psize; auto].
+ intros (H,_); compute in H; elim H; auto.
+Qed.
+
+Lemma addmuldiv_spec : forall x y p, [|p|] <= [|digits|] ->
+   [| addmuldiv p x y |] =
+   ([|x|] * (2 ^ [|p|]) + [|y|] / (2 ^ ([|digits|] - [|p|]))) mod wB.
+Proof.
+(*** WARNING : TODO *)
+Admitted.
+
+Lemma head00_spec:  forall x, [|x|] = 0 -> [|head0 x|] = [|digits|].
+Proof. 
+ change 0 with [|0|];intros x Heq.
+ apply to_Z_inj in Heq;rewrite Heq;trivial.
+Qed.
+
+Lemma tail00_spec:  forall x, [|x|] = 0 -> [|tail0 x|] = [|digits|].
+Proof.
+ change 0 with [|0|];intros x Heq.
+ apply to_Z_inj in Heq;rewrite Heq;trivial.
+Qed.
+
+
+
+
